# PDFæ–‡æ¡£å†…å®¹æå–
> æå–æ—¶é—´: 2025-09-18 23:03:12
> æ€»é¡µæ•°: 4
> å¤„ç†é¡µæ•°: 4

## ç¬¬ 1 é¡µ

[OPENAI_EXTRACTION_FAILED]

---

## ç¬¬ 2 é¡µ

[OPENAI_EXTRACTION_FAILED]

---

## ç¬¬ 3 é¡µ

2 Fundamentals of Inequalities April 16, 2022

The quantity P(r) is called the rth power mean. Note that if we set all the weights equal, that is wâ‚ = wâ‚‚ = ... = w = 1, then
To save the space, we will introduce three tricks from the pre-pages.
1. product!
P(r) = (aâ‚ + aâ‚‚ + ... + aâ‚™ / n)Â¹/r râ‰ 0
If it says abc=1. we can let a = x/y, b = y/z, c = z/x, w.l.o.g. r=0.
Corollary 2.7 (QM-AM-GM-HM theorem). Let aâ‚, ..., aâ‚™ be positive real numbers. Then
2. Ravi substitution
âˆš(aâ‚Â² + ... + aâ‚™Â²) / n â‰¥ (aâ‚ + ... + aâ‚™) / n â‰¥ â¿âˆš(aâ‚aâ‚‚...aâ‚™) â‰¥ n / (1/aâ‚ + ... + 1/aâ‚™)
If a.b.c are three sides of a triangle, we can replace ca, b, a
Proof. Set r âˆˆ {2,1,0,-1} we obtain the inequality
with (x+y, y+z, z+x)
Here "QM" and "HM" stand for "quadratic mean" and "harmonic mean"
Here is an application of a â…“-power mean. âˆ‘ cyc aÂ²(caÂ²+bc) â‰¥ âˆ‘ cyc a^(r+1) c(b+c)
3. Schur inequality
Example 14 (Taiwan TST 2014). Let a, b, c > 0. Prove that
When r=1, that's the common form we use:
3(a+b+c) â‰¥ 8âˆ›abc + âˆš(aÂ³ + bÂ³ + cÂ³) / 3
aÂ³+bÂ³+cÂ³ + 3abc â‰¥ âˆ‘ cyc aÂ²b

Solution 14. By Power Mean with r = 1, s = â…“, and weights 1/9 + 8/9 = 1 we have the inequality
(1/9 âˆš(aÂ³ + bÂ³ + cÂ³) / 3 + 8/9 âˆ›abc)Â³ â‰¤ 1/9 (aÂ³ + bÂ³ + cÂ³) / 3 + 8/9 (abc).
Thus it is enough to prove aÂ³+bÂ³+cÂ³+24abc â‰¤ (a+b+c)Â³, which is clear.
â†’ Example: (aÂ²+bÂ²)(cÂ²+dÂ²) â‰¥ (ac+bd)Â²

Â§2.4.2 Cauchy and HÃ¶lder vector form: |a|â‹…|b| â‰¥ |aâ‹…b|
We now present HÃ¶lder's inequality; we state the two-variable form for concreteness but the obvious generalization to any number of sequences is valid.

Theorem 2.8 (HÃ¶lder's inequality). Let p and q be positive real numbers. Let aâ‚, ..., aâ‚™, bâ‚, ..., bâ‚™ be nonnegative real numbers. Then
(âˆ‘áµ¢â‚Œâ‚â¿ aáµ¢áµ–)Â¹/áµ– (âˆ‘áµ¢â‚Œâ‚â¿ báµ¢q)Â¹/q â‰¥ (âˆ‘áµ¢â‚Œâ‚â¿ áµ–âºqâˆšaáµ¢áµ–báµ¢q)Â¹/(p+q)
When p=q=1, that is Cathy's inequality:
âˆ‘áµ¢â‚Œâ‚â¿ aáµ¢ â‹… âˆ‘áµ¢â‚Œâ‚â¿ báµ¢ â‰¥ (âˆ‘áµ¢â‚Œâ‚â¿ âˆšaáµ¢báµ¢)Â²
25

---

## ç¬¬ 4 é¡µ

2 Fundamentals of Inequalities April 16, 2022

Solution 16. This time, we use HÃ¶lder with slightly changed weights in order to remove the square root:

(âˆ‘ğ‘/âˆšğ‘+ğ‘)2(âˆ‘ğ‘(ğ‘+ğ‘))â‰¥(ğ‘+ğ‘+ğ‘)3.
ğ‘ğ‘¦ğ‘ ğ‘ğ‘¦ğ‘

Again it is enough to prove (ğ‘+ğ‘+ğ‘)2â‰¥3âˆ‘ğ‘ğ‘¦ğ‘ğ‘(ğ‘+ğ‘) which is true by expanding.

Exercise. Show that if one sets ğ‘ğ‘–=1 for each ğ‘–, then HÃ¶lder's inequality reduces to a power mean inequality with all weights equal.

Â§2.5 Inequalities in arbitrary functions

Let ğ¼ be an open interval (for example ğ¼=(0,âˆ) or ğ¼=(0,1)) and let ğ‘“:(ğ‘¢,ğ‘£)â†’â„ be a function and let ğ‘1,ğ‘2,...,ğ‘ğ‘›âˆˆ(ğ‘¢,ğ‘£). Suppose that we fix ğ‘1+ğ‘2+...+ğ‘ğ‘›=ğ‘ (if the inequality is homogeneous, we will often insert such a condition) and we want to prove that

ğ‘“(ğ‘1)+ğ‘“(ğ‘2)+...+ğ‘“(ğ‘ğ‘›)

is at least (or at most) ğ‘›ğ‘“(ğ‘). In this section we will provide two methods for doing so.

Definition 2.10. We say that function ğ‘“ is convex if the second derivative ğ‘“â€²â€² is nonnegative over all of (ğ‘¢,ğ‘£). Similarly we say it is concave if ğ‘“â€²â€²(ğ‘¥)â‰¤0 for all ğ‘¥. Note that ğ‘“ is convex if and only if âˆ’ğ‘“ is concave.

Let ğ‘>0, ğ‘>0, 1/ğ‘+1/ğ‘=1, ğ‘“(ğ‘¥)=ln(ğ‘¥), then 1/ğ‘lnğ‘¥+1/ğ‘lnyâ‰¤ln(ğ‘ğ‘¥+ğ‘ğ‘¦)
Â§2.5.1 Jensen and Karamata i.e. ğ‘¥1/ğ‘ğ‘¦1/ğ‘â‰¤ğ‘ğ‘¥+ğ‘ğ‘¦

We have the following analog of AM-GM now.

Theorem 2.11 (Jensen's inequality). Let ğ‘“:ğ¼â†’â„ be a convex function. Then for any ğ‘1,...,ğ‘ğ‘›âˆˆğ¼ we have

åŠ æƒ: ğ‘“(ğ‘1)+...+ğ‘“(ğ‘ğ‘›)/ğ‘›â‰¥ğ‘“(ğ‘1+...+ğ‘ğ‘›/ğ‘›).
ğ‘1ğ‘“(ğ‘¥1)+...+ğ‘ğ‘›ğ‘“(ğ‘¥ğ‘›)â‰¤ğ‘“(ğ‘1ğ‘¥1+...+ğ‘ğ‘›ğ‘¥ğ‘›).

The reverse inequality holds when ğ‘“ is concave.

Exercise. Show that if one takes ğ¼=(0,âˆ) and ğ‘“ to be the natural logarithm, then Jensen reduces to AM-GM with all weights equal.

Just as Muirhead is repeated AM-GM, there is an analog of repeated Jensen; however its use is somewhat rarer.

Theorem 2.12 (Karamata's inequality). Let ğ‘“:ğ¼â†’â„ be convex. Suppose the sequence (ğ‘¥ğ‘›) majorizes (ğ‘¦ğ‘›), with each ğ‘¥ğ‘– and ğ‘¦ğ‘– in ğ¼. Then

å‚è§å‰æ–‡"Î»" ğ‘“(ğ‘¥1)+...+ğ‘“(ğ‘¥ğ‘›)â‰¥ğ‘“(ğ‘¦1)+...+ğ‘“(ğ‘¦ğ‘›).

The reverse inequality holds when ğ‘“ is concave.

27

---

